---
title: Comp2711
category: Study
tags: [ comp2711 ]
date: 2016-10-17
filename: 2016-10-17-Comp2711
---

## L2

- Product Principle: if a set of lists of length $m^I$ has the properties below, then there are $prod^m_{k=1} i_k$ lists in S
  - there are i different elements of lists in S, and
  - for each j $>$ i, and each choice of j-1 elements of a list in S, there are $i_j$ choice of elements in position j of those lists
- function (F): relationship between two lists (can point from multiple elements from one set to only one element to other set)
- function (F) is one-to-one/injection if $(x != y) \Longrightarrow (f(x) != f(y))$
- function (F) is onto/surjection if all f(y) gets a arrow pointing at it
- function (F) is bijection/one-to-one correspondance if it is both one-to-one and onto

## L3

- increasing triples i.e. i,j,k where i <= j <= k, is same as 3-element subsets

- $\begin{pmatrix}n \\k\end{pmatrix}$

  $ = \frac{n!}{k!(n-k)!}$

## L4

- $\sum_{i=0}^{4}\begin{pmatrix} n \\ i \\\end{pmatrix} =2^n$
- Pascal relationship: each element in Pascal's triangle is equal to sum of two elements above it i.e. $\binom{3}{2}=\binom{2}{1}+\binom{2}{2}$

## L5

- Coeficient of a term e.g. $x^3y^2z^3$ in $(x+y+z)^8$ is $\begin{pmatrix} 8 \\ 3 \end{pmatrix}*
  \begin{pmatrix} 8 \\ 2 \end{pmatrix}*
  \begin{pmatrix} 8 \\ 3 \end{pmatrix} $

## L6

### Fermet's Little theorem

- if p is a prime, then $a^{p-1}$ mod p=1 for each nonzero a

### Implies

- 'implies': $\implies$. Just like a promise, if i didnt say true, even if u got false i didnt broke the promise.

| s    | t    | s$\implies$t |
| :--- | :--- | :----------- |
| T    | T    | T            |
| T    | F    | F            |
| F    | T    | T            |
| F    | F    | T            |

### Universe i.e. wildcard

- for getting certain exceptions/everything included

#### Exist symbol: $\exists$

- = there exists something that satisfies a condition

#### All symbol: $\forall$

- = all things satisfies a condition

## L7

#### $U_1 = \{x \exists U_2 | q(x) is true\}$

- Put it simple, smaller universes inherits the logics from larger universe
- Anything that can be interpreted about $U_1$ can be interpreted about $U_2$
- $\forall X \exists U_1 (p(x))$ is same as $\forall X \exists U_2 (q(x) \implies p(x))$
- $\exists X \exists U_1 (p(x))$ is same as $\exists X \exists U_2 (q(x) \land p(x))$

#### 4.3: $\neg \forall X \exists U(p(x))$ = $\exists X \exists U(\neg p(x))$

- not all to exist
- Put it simple, if not all of the people are boys, then there are girls

#### 4.4:  $\neg \exists X \exists U(p(x))$ = $\exists X \exists U(\neg p(x))$

- not exist to all
- Kind of same as before

### Infernce

- for proving stuff

#### Direct inference

For p and p $\implies$q, we may conclude q

#### Direct Proof

- Consists of a sequence of statements, either a hypothtesis, fact or resolt of rules of inference or compound statements

#### Indirect Proof

##### Contrapositive rule of inference

e.g. $\neg q \implies \neg p$ is contrapositive of $p \implies q$
**DOESNT** mean $p \implies q$

## T2

### Test 1

- 6 rings on 10 fingers:
  - rings are different: $10^6$
  - rings are sase: $10C6$

## L8

### Strong principle of Mathematicial induction

- if state p(b) is true and
- for all n $>$ b, the statement p(b) $\land$ p(b+1) $\land$ ... $p(n-1)$ $\Rightarrow$ p(n) is true
  - then p(n) is true for all integers n $n>=$b

#### E.g. prove that every positive integer is a power of a primer or the product of powers of prime numbers

- base case: 1 is a power of a prime number
- inductive hypothesis: suppose that we know that every number less than n is a power of a prime number or a product of powers of prime number.
  - case 1: n is a prime number. Then itself is its factor
  - case 2: n is not a prime number. Then n=$k_1k$

### Hashing

- unique ID assignment to 'mailboxes', tries to make each mailbox has evenly distributed mails received, while keeping randomness

### Probability Theory

#### Define Three related but different concepts:

- Underlying sample spacee and elements(outcomes) in the sample space
- An event in the sample space
- The Weight of an element in the sample space gives a probability distibution

##### Event: a subsets of outcomes in outerspace (outcomes that have have common features)

##### Weight: probability of each possible combination, sum of all weights = 1



## L10

### Conditional Probability

- e.g. Given two dices are thrown and sum is 4, what is the probability of double 2's.
- Makes the given condition 1 since it has already happened
- = absolute of the question $\times$ 1/ (<probabiity of the given condition if it had not been guaranteed to happen >)
- e.g. P(sum is even | sum $\geqslant$ 10) i.e. given sum is bigger than or equal to 10, probability of sum being even =$\frac{P(sum\ is\ even \lor sum \geqslant 10)}{P(sum \geqslant 10)}$

### ==MID TERM==

1. Counting:
   1. sum priciple
   2. product principle
   3. $\begin{pmatrix}n\\k\end{pmatrix}$ products of binomial coefficient i.e. Pascal Triangle
2. Logic:
   1. Truth tables
   2. To prove 2 statements are logiclly equivalent
      1. Truth tables
      2. Demogan's law, Distriibutive law, Associative law, etc.
      3. a $\Rightarrow$ b $\equiv$ $\neg a \lor b$
3. Quantifiers: $\forall, \exists$ e.g. Theorem 3.2 in quantifier lecture note
4. Inference
   1. Direct inference p(x) 
   2. Contrapositive
   3. Contradiction
5. Probability
   1. Intro to Probability
   2. Includion & exclusion ($P \lor E_1 \lor E_2 \lor E_3 ...$)
   3. Complementing E and F i.e. P(E) = 1 - P(F)
6. M.I.
   1. Base case
   2. P(n)
   3. Prove P(n+1)
   4. p(n) $\rightarrow$ p(n+1), by the principle of M.I....

## L11

#### Relation of independent trials

- e.g. Probability of 'H on i^th^ flip' is $\frac{1}{2}$

  Probability of 'H on i^th^ flip', given a particular sequence on first i-1 flips, is still $\frac{1}{2}$

- to hashing tho:
  P(key i hashes to r) = $k^{-1}$
  P(key i hashes to r $\land$ keys 1 through i-1 hash to $q_1, q_2, ....q_{i-1}$) = $k^{-i}$
  P(keys 1 through i-1 hash to $q_1, q_2, ....q_{i-1}$) = 

##### Bernouli trial: Trials that is either success or fail

## L12

#### Expected value E(X) = $\sum_{i=1}^k x_i P(X=x_i)$

## L13

##### 'indicator random variable': random variable that is boolean

##### 'linearity of expectation': e.g. n students pick from a pile of bags, probability of each student getting their bag (X) = $x_1+x_2+x_3+...$

##### 'Expected number of trials til a probability': 1/ (All possibilities)

#### If X is random variable that always take on value , then E(X) =c

#### If X is random variable in sample space, then E(E(X)) = E(X)

#### V(X) ('variance') = E(X-E(X))$^2$

### Variance

##### Variance of a sum of independent R.V.s is sum of their variances V(XY) = V(X)+ V(Y)

#### e.g. Variance for 10 coin flips:

since variance for 1 coin flip is 1/4, its just 10$\cdot$ 1/4= 2.5

##### Variance for bernoulli trials(i.e. boolean), variance = np(1-p)

##### 1 Standard Deviation = $\sqrt{variance}$

## L14

### Crypto

#### Private-Key cryptography

Sender and receiver agree in advance on a secret and then send messages using that code

##### Ceasar Cipher

Use [0,1,....] for [A,B,...]

Convert message to sequence of numbers

play with the sequence such as shifting, mod

> not that safe

##### Crypography using multiplication mod n

Multiplies message with some a, then mod some n

Need to make sure encrypted stuff can be decrypted to be unique

## L15

#### Public-key Cryptosystems

No agreement in advance on secret code

Each user have a public key and a private key

##### To make it safe (result is RSA Public Key Cryptosystem):

- Make it easy for receiver with private key to calculate the message
- Make it hard for hard to derive private key from public key

### Inverse and GCDs

##### Prove, by contradiction that m=qn+r

Assume that there is a non-negative m which the statement fails
choose smallest m for which q,r satisfying the statement does not exist

If m < n, then m= 0$\cdot$ n + m so it is satisfied with q=0, r=m which contradicts.
If m >= n, then m-n >= 0. Then m-n = n$q_1+r_1​$ . Adding n to both sides will get  m = n$q_1+n+r_1​$ , which contradicts also.



------

- #### bla bla GCD theorem

  - ​

```cpp
int gcd(int k,int j) { // j < k
  if (!j) return k;
  return gcd(j, k%j);
}
```

- ###### Extended GCD theorem

- ​

  - Return x and y also, such that gcd(j,k) = jx+ky
  - Proof:
    - base case: since the result of gcd will be j, to make j=jx+ky we set x=1 and y=0
    - non-base case: recursively compute ==gcd(r,j)=rx'+jy', where y = x' and x = y' - qx'==

- Computing inverse with extended GCD theorem

  given  a =27, n = 58. find that 27(-15)+58(7)=1. Since -15 is not within the range, one extra step: -15 mod 58 = 43 is the multiplicative inverse of 27 in $Z_{58}$

- #### Multiplicative inverse

  - Using multiplicative inverse in encryption: $a \cdot$~n~ x=b. x is original message, b is encrypted message
  - if a$\cdot _n x =b$ have solution for all b $\in$ Z, then $x=a' \cdot _n b$ i.e. a have inverse $\in$ Z
  - if a and n are relatively prime $\Leftrightarrow$ a has inverse
  - Converting modular equation t normal equation:
    $a\cdot _n x=1$ has solution // a has inverse in $Z_n$ only if has an integer x,y where ax+ny = 1
    $a\cdot _n x=(ax+ny)$ mod n (lemma 2.9)
  - to be remembered: theorem 2.9, corollary 2.10, lemma 2.11
  - ​

- If p is prime number, $\forall$ a $\in Z_p$, $a^{p-1} mod p = 1$ or for every positive interger a not multiple of p
  - Prove that the or thing works: $a^{p-1} mod p = 1 $\Leftrightarrow (lemma 2.3) $(a mod p)^{p-1}$ mod p = 1
- $a^m$ mod p = $a^{m mod(p-1)} mod p 
  - Proof: $a^m$ mod p = $a^{n(p-1)}\cdot a^{m mod(p-1)} mod p$ = $(a^{p-1} mod p)^n \cdot a^{m mod (p-1)} mod p = a^{m mod (p-1)} mod p$
-  ​
- ####  RSA
  - Key choice algorithm
    1. choose 2 large prime numbers p and q that are large
    2. set n =pq and T = (p-1)(q-1)
    3. Choose e != 1 s.t. gcd(e, T) = 1
    4. Calculate d = $e^{-1} mod T$ (e is for encryption, d is for decryption)
    5. Publish e,n as public key
    6. Kepp d as private key
    To get private message: take x as message, x = ($x^{ed} mod n)
  - Proof:
    1. Prove that x mod p = $x^{ed} mod p$
      p, q be primes
      n = pq
      T = (p-1)(q-1)
      d = $e^{-1} mod T$
      ed = Tk + 1
         = (p-1)(q-1)k+1
         $\implies$ $x^{(p-1)(q-1)k+1}$ mod p
      Two possible cases:
        1. $x^{k(q-1)} is multiple of p, then x must be multiple of p as well, then = x mod p since both are 0s
        2. otherwise, then it is right as well
    2. Prove that x mod q = $x^{ed} mod q$, same as (1)
    3. Prove that x = $x^{ed} mod n$, combine above mod equations and will easily get
