---
title: Math2111
desc: L
category: Study
tags: [ math2111 ]
date: 2016-11-17
filename: 2016-11-17-Math2111
---

[](http://ihome.ust.hk/~makywong/Week%2012%20Notes.pdf)

# Math2111

If S is an orthogonal set of non-zero vectors then S is L.I.

==Orthonormal basis==: normalization form of orthogonal basis

Matrix A is orthogonal if $A^T A$ = 1 $\Leftrightarrow$ columns of A form orthonormal  basis of $R^n$ $\Leftrightarrow$ rows of $A^T$ form orthonormal basis of $R^n$

For x,y $\in R^n$, and U is matrix consisting of orthonormal columns then ||Ux|| = ||x1|| 

==Orthogonal projection== (like shadows): Need to find proj$_wv$ i.e. shadow

1. Find an orthogonal basis of W {$v_1, v_2, ...$} 


2. proj$_wv$ = $\frac{v\cdot v_1}{v_1\cdot v_1}v_1$+...

==Recipe for Orthogonal projection from Span W==

>  Example (P.7):

1. find orthogonal basis of W
2. Since is linearly independent, dim W = 2. So find 2 orthogonal vectors in W , are {$\begin{pmatrix}1\\0\\0\end{pmatrix}, \begin{pmatrix}0\\1\\0\end{pmatrix}$} 

proj$_wv$ = $\frac{v\cdot v_1}{v_1\cdot v_1}v_1 + ..$ , with v = $\begin{pmatrix}x\\y\\z\end{pmatrix}$, get proj$_wv$ = $\begin{pmatrix}x\\y\\0\end{pmatrix}$

> Example #a w = span{$\begin{pmatrix}1\\2\\2\end{pmatrix}\begin{pmatrix}-2\\2\\-1\end{pmatrix}$}, v = $\begin{pmatrix}3\\2\\-5\end{pmatrix}$

1. dim W =2. The 2 Orthogonal vectors are columns of w
2. proj$_wv$ = $\begin{pmatrix}-1\\0\\-1\end{pmatrix}$

==2nd Recipe for Orthogonal projection from Span W==

1. Find orthonormal basis of W 
2. U = ($v_1, ...$). $UU^T$ is the projection matrix
3. proj$_wv$ = ($UU^T$)v

> Example (revisit #a)

1. Still find orthogonal basis of w
2. U = orthogonal basis of w, find $UU^T$
3. proj$_wv$ = $UU^T$ v = $UU^T \begin{pmatrix}3\\2\\-5\end{pmatrix}$ = $\begin{pmatrix}-1\\0\\-1\end{pmatrix}$

Why the recipes work

​	Need to prove the formula proj$_wv$ = $\frac{v\cdot v_1}{v_1\cdot v_1}v_1+....$

​		Need to prove for v - proj$_wv \in$ $w^{\perp}$, v - proj$_wv \cdot v_{1\ to\ p}$ =0

​		$V_1 ( v - $proj$_wv$)$ = $$v_1 v + v_1 (\frac{v\cdot v_1}{v_1\cdot v_1}v_1+ ...)$ = ... = $v_1 v - v_1 v$ = 0

 